Add test

test.lean
@@ -3,9 +3,97 @@ def some_lets : ℕ → ℕ → ℕ
 | 0            v := v
 | (nat.succ n) v := let k := some_lets n v + some_lets n v in some_lets n k
 
-def some_unfolded_lets (n : ℕ) : ∃ v : ℕ , v = some_lets 5 n :=
+def some_unfolded_lets (n : ℕ) : Σ' v : ℕ , v = some_lets 5 n :=
 begin
-  unfold some_lets; constructor; constructor
+  constructor; unfold some_lets; constructor
 end
 
-#print some_unfolded_lets
+universe variables u v
+inductive let_inM : Sort u → Sort (u+1)
+| ret : Π {A : Sort u} , A → let_inM A
+| bind : Π {A : Sort u} {B : Sort u} , let_inM A → (A → let_inM B) → let_inM B
+| app2 : Π {A B C : Sort u} , (A → B → C) → let_inM A → let_inM B → let_inM C
+
+def denote_let_inM : Π {A : Sort (u+1)} , let_inM A → A
+| A (@let_inM.ret ._ v) := v
+| B (@let_inM.bind A ._ v f) := let v' := @denote_let_inM A v in @denote_let_inM B (f v')
+| C (@let_inM.app2 A B ._ f x y) := f (denote_let_inM x) (denote_let_inM y)
+attribute [simp] denote_let_inM
+
+def under_lets : Π {A B : Sort (u+1)} , let_inM A → (A → let_inM B) → let_inM B
+| A B (@let_inM.ret ._ v) f := let_inM.bind (let_inM.ret v) f
+| A B (@let_inM.bind A2 ._ v g) f := under_lets v (λ v' , under_lets (g v') f)
+| A B (@let_inM.app2 A2 B2 ._ g x y) f := under_lets x (λ x' , under_lets y (λ y' , f (g x' y')))
+attribute [simp] under_lets
+
+def lift_lets : Π {A : Sort (u+1)} , let_inM A → let_inM A :=
+  λ A v , @under_lets A A v (@let_inM.ret _)
+
+lemma denote_under_lets_correct {A : Sort (u+1)} {B : Sort (u+1)} (v : let_inM A)
+ : ∀ (f : A → let_inM B), @denote_let_inM B (@under_lets A B v f) = @denote_let_inM B (f (@denote_let_inM A v)) :=
+begin
+  induction v; intro f; try { reflexivity }; simp; rewrite ih_1; rewrite ih_2
+end
+lemma lift_lets_correct {A : Sort (u+1)} (v : let_inM A)
+ : denote_let_inM v = denote_let_inM (lift_lets v)
+:= by symmetry; apply denote_under_lets_correct
+
+meta def reify_to_let_in_pexpr_aux : expr → (pexpr → pexpr) → pexpr
+| (expr.elet n ty val body) f := let val' := reify_to_let_in_pexpr_aux val (λ x, ``(@let_inM.ret _ %%x)) in
+                                 let body' := reify_to_let_in_pexpr_aux body f in
+                                 let body' := expr.lam n binder_info.default (pexpr.of_expr ty) body' in
+                                 ``(@let_inM.bind %%ty _ %%val' %%body')
+| `(%%a + %%b) f := let a' := reify_to_let_in_pexpr_aux a (λ x, ``(@let_inM.ret _ %%x)) in
+                    let b' := reify_to_let_in_pexpr_aux b (λ x, ``(@let_inM.ret _ %%x)) in
+                    ``(@let_inM.app2 _ _ _ (λ a' b' , a' + b') %%a' %%b')
+| e f := f (pexpr.of_expr e)
+
+meta def reify_to_let_in_pexpr (e : expr) : pexpr := reify_to_let_in_pexpr_aux e (λ x , ``(@let_inM.ret _ %%x))
+
+
+meta def is_eq : expr → option (expr × expr × expr)
+| `(@eq %%α %%a %%b) := some (α, a, b)
+| _                  := none
+
+open tactic
+meta def unify_reify_rhs_to_let_in : tactic unit :=
+  do [g] <- tactic.get_goals,
+     gl_ty <- tactic.infer_type g,
+     match is_eq gl_ty with
+     | some (ty, ev, v)
+        := let v' := reify_to_let_in_pexpr v in
+           let v' := ``(denote_let_inM %%v') in
+           do _ <- tactic.refine ``(@eq.trans _ _ %%v' _ _ (eq.refl _)),
+              (g0 :: g :: []) <- tactic.get_goals,
+              tactic.set_goals [g]
+     | none := tactic.fail "not an equality"
+     end
+
+-- set_option debugger true
+open tactic
+def some_lifted_lets (n : ℕ) : Σ' (v : ℕ), v = psigma.fst (some_unfolded_lets n) :=
+begin
+  constructor; unfold some_unfolded_lets psigma.fst; symmetry; transitivity; symmetry,
+  {
+    unify_reify_rhs_to_let_in; symmetry; to_expr ``(lift_lets_correct) >>= apply
+  },
+  {
+     symmetry; transitivity; symmetry,
+     {
+       unfold lift_lets under_lets; constructor
+      },
+     { unfold denote_let_inM; constructor }
+  }
+
+end
+
+
+
+
+-- #print some_unfolded_lets
+/-
+#print reify_to_let_in_pexpr
+#print expr
+#print let_inM
+#print binder_info-/
+-- #print some_unfolded_lets
